swticing to FSet based implementation (unfinished)

coq/SigmaHCOL/Memory.v
@@ -4,9 +4,14 @@
   Memory cells all have the same type: `CarrierA`.
  *)
 
-Require Import Coq.FSets.FMapAVL.
-Require Export Coq.FSets.FMapInterface.
-Require Import Coq.FSets.FMapFacts.
+From Coq.FSets Require Import
+     FSetAVL
+     FSetInterface
+     FSetFacts
+     FMapAVL
+     FMapInterface
+     FMapFacts.
+
 Require Import Coq.Structures.OrderedTypeEx.
 Require Import Coq.Arith.Peano_dec.
 
@@ -14,6 +19,7 @@ Require Import ExtLib.Structures.Monads.
 Require Import ExtLib.Data.Monads.OptionMonad.
 
 Require Import Helix.HCOL.CarrierType.
+Require Import Helix.Tactics.HelixTactics.
 
 Import MonadNotation.
 Open Scope monad_scope.
@@ -35,9 +41,12 @@ Proof.
 Qed.
 
 Module NM := FMapAVL.Make(Nat_as_OT).
+Module Import NF := FMapFacts.WFacts_fun(Nat_as_OT)(NM).
 Definition NatMap := NM.t.
 
-Module Import NF:=WFacts_fun(Nat_as_OT)(NM).
+Module NS := FSetAVL.Make(Nat_as_OT).
+Module Import NSF := FSetFacts.WFacts_fun(Nat_as_OT)(NS).
+Definition NatSet := NS.t.
 
 Definition mem_add k (v:CarrierA) := NM.add k v.
 Definition mem_delete k (m:NatMap CarrierA) := NM.remove k m.
@@ -52,53 +61,42 @@ Definition mem_block := NatMap CarrierA.
 Definition mem_keys (m:NatMap CarrierA): list nat
   := List.map fst (NM.elements m).
 
-(* Copy of template-coq `monad_fold_left` but using ExtLib
-   TODO: move to Util
-*)
-Fixpoint monadic_fold_left
-         {A B:Type}
-         {m : Type -> Type}
-         {M : Monad m}
-         (f : A -> B -> m A) (l : list B) (x : A)
-  : m A
-  := match l with
-     | nil => ret x
-     | y :: l => x' <- f x y ;;
-                  monadic_fold_left f l x'
-     end.
+Definition mem_keys_lst (m:NatMap CarrierA): list nat :=
+  List.map fst (NM.elements m).
 
-Fixpoint monadic_fold_left_rev
-         {A B:Type}
-         {m : Type -> Type}
-         {M : Monad m}
-         (f : A -> B -> m A) (l : list B) (x : A)
-  : m A
-  := match l with
-     | nil => ret x
-     | y :: l => x' <- monadic_fold_left_rev f l x ;; f x' y
-     end.
+Definition mem_keys_set (m: mem_block): NatSet :=
+  List.fold_right NS.add NS.empty (mem_keys_lst m).
 
-Definition mem_try_add (m:mem_block) '(k,v) :=
-  match NF.In_dec m k with
-  | left _ => None
-  | right _ => Some (NM.add k v m)
-  end.
+(* forcefull union of two memory blocks. conflicts are resolved by
+   giving preference to elements of the 1st block *)
+Definition mem_union (m1 m2 : mem_block) : mem_block
+  := NM.map2 (fun mx my =>
+                match mx with
+                | Some x => Some x
+                | None => my
+                end) m1 m2.
 
-(* merge two memory blocks. Return `None` if there is an overlap *)
+Definition is_disjoint (a b: NatSet) : bool :=
+  NS.is_empty (NS.inter a b).
+
 Definition mem_merge (a b: mem_block) : option mem_block
-  := monadic_fold_left_rev mem_try_add
-       (NM.elements a) b.
+  :=
+    let kx := mem_keys_set a in
+    let ky := mem_keys_set b in
+    if is_disjoint kx ky
+    then Some (mem_union a b)
+    else None.
 
 (* merge two memory blocks in (0..n-1) using given operation to combine values *)
-Definition mem_merge_with (f: CarrierA -> CarrierA -> CarrierA) (a b: mem_block)
-  : mem_block
+Definition mem_merge_with (f: CarrierA -> CarrierA -> CarrierA): mem_block -> mem_block -> mem_block
   :=
-    NM.fold (fun k v m =>
-               match mem_lookup k m with
-               | None => NM.add k v m
-               | Some x => NM.add k (f v x) m
-               end
-            ) a b.
+    NM.map2 (fun a b =>
+               match a,b with
+               | None, None => None
+               | Some x, None => Some x
+               | None, Some y => Some y
+               | Some x, Some y => Some (f x y)
+               end).
 
 (* block of memory with indices (0..n-1) set to `v` *)
 Fixpoint mem_const_block (n:nat) (v: CarrierA) : mem_block
@@ -111,3 +109,131 @@ Fixpoint mem_const_block (n:nat) (v: CarrierA) : mem_block
 Definition memory := NatMap mem_block.
 
 Definition mem_block_equiv:= NM.Equal (elt:=CarrierA).
+
+(* ------------------ Proofs below ------------------- *)
+
+Lemma NF_eqb_eq {a b: nat}:
+  NF.eqb a b = true -> a = b.
+Proof.
+  intros H.
+  unfold NF.eqb in H.
+  break_if.
+  - auto.
+  - inversion H.
+Qed.
+
+Lemma NF_eqb_neq {a b: nat}:
+  NF.eqb a b = false -> a <> b.
+Proof.
+  intros H.
+  unfold NF.eqb in H.
+  break_if.
+  - inversion H.
+  - auto.
+Qed.
+
+Lemma mem_block_as_fold_right (m:mem_block):
+  NM.Equal m
+           (List.fold_right
+              (fun '(k,v) m' => NM.add k v m')
+              mem_empty
+              (NM.elements m)).
+Proof.
+Admitted.
+
+
+Lemma mem_keys_set_In (k:NM.key) (m:mem_block):
+  NM.In k m <-> NS.In k (mem_keys_set m).
+Proof.
+  pose proof (NM.elements_3w m) as U.
+  split; intros H.
+  -
+    rewrite mem_block_as_fold_right with (m:=m) in H.
+    unfold mem_keys_set, mem_keys_lst.
+    generalize dependent (NM.elements m). intros l U H.
+    induction l.
+    +
+      simpl in H.
+      apply empty_in_iff in H.
+      tauto.
+    +
+      destruct a as [k' v].
+      simpl in *.
+      destruct (eq_nat_dec k k') as [K|NK].
+      *
+        (* k=k' *)
+        apply NS.add_1.
+        auto.
+      *
+        (* k!=k' *)
+        apply add_neq_iff; try auto.
+        apply IHl.
+        --
+          inversion U.
+          auto.
+        --
+          eapply add_neq_in_iff with (x:=k').
+          auto.
+          apply H.
+  -
+    rewrite mem_block_as_fold_right with (m:=m).
+    unfold mem_keys_set, mem_keys_lst in H.
+    generalize dependent (NM.elements m). intros l U H.
+    induction l.
+    +
+      simpl in H.
+      apply empty_iff in H.
+      tauto.
+    +
+      destruct a as [k' v].
+      simpl in *.
+      destruct (eq_nat_dec k k') as [K|NK].
+      *
+        (* k=k' *)
+        apply add_in_iff.
+        auto.
+      *
+        (* k!=k' *)
+        apply add_neq_in_iff; auto.
+        apply IHl.
+        --
+          inversion U.
+          auto.
+        --
+          apply NS.add_3 in H; auto.
+Qed.
+
+Lemma mem_keys_set_in_union_dec
+      (m0 m1 : mem_block)
+      (k : NM.key):
+  NS.In k (mem_keys_set (mem_union m0 m1)) ->
+  {NS.In k (mem_keys_set m1)}+{NS.In k (mem_keys_set m0)}.
+Proof.
+  intros H.
+  unfold mem_union in H.
+  apply mem_keys_set_In, NM.map2_2 in H.
+  rewrite 2!mem_in_iff in H.
+  apply orb_true_intro, orb_true_elim in H.
+  inversion H; [right|left] ;
+    apply mem_keys_set_In, mem_in_iff;
+    auto.
+Qed.
+
+Lemma mem_merge_key_dec
+      (m m0 m1 : mem_block)
+      (MM : mem_merge m0 m1 = Some m)
+  :
+    forall k, NM.In k m -> {NM.In k m0}+{NM.In k m1}.
+Proof.
+  intros k H.
+  rename m into mm.
+  destruct (NF.In_dec m1 k) as [M1 | M1], (NF.In_dec m0 k) as [M0|M0]; auto.
+  exfalso. (* Could not be in neither. *)
+  unfold mem_merge in MM.
+  break_if; inversion MM.
+  subst mm. clear MM.
+  rewrite mem_keys_set_In in M0, M1.
+  clear Heqb.
+  apply mem_keys_set_In, mem_keys_set_in_union_dec in H.
+  destruct H; auto.
+Qed.
